Eff.Equation.Test2.fst
@@ -74,28 +74,33 @@ let st_eq : template_equation rw
 
 assume val a : Type
 
-let h1_raw : handler_raw rw [] a rw []
-  = fun op x k -> let y = perform op x in k y
-  
-let h1 : handler rw [] a rw []
-  = (| h1_raw , () |)
 
-let h2_raw : handler_raw rw [] a rw [st_eq3]
-  = fun op x k -> let y = perform op x in k y
+let h1 : handler rw [] a rw [] = {
+  op_cases = (fun op x k -> let y = perform op x in k y);
+  respects = ()
+}
 
-let h2 : handler rw [] a rw [st_eq3]
-  = (| h2_raw , () |)
+let h2 : handler rw [] a rw [st_eq1;st_eq2;st_eq3] = {
+  op_cases = (fun op x k -> let y = perform op x in k y);
+  respects = ()
+}
 
-let h3_raw : handler_raw rw [] a rw [st_eq2]
-  = fun op x k -> let y = perform op x in k y
+let h3 : handler rw [st_eq] a rw [st_eq1;st_eq2;st_eq3] = {
+  op_cases = (fun op x k -> let y = perform op x in k y);
+  respects = (fun () -> ())
+}
 
-let h3 : handler rw [] a rw [st_eq2]
-  = (| h3_raw , () |)
+let h4 : handler rw [st_eq;st_eq] a rw [st_eq1;st_eq2;st_eq3] = {
+  op_cases = (fun op x k -> let y = perform op x in k y);
+  respects = (fun () -> ()) , (fun () -> ())
+}
 
+
+
+(*
 let h4_raw : handler_raw rw [st_eq] a rw [st_eq3]
   = fun op x k -> let y = perform op x in k y
 
-(*
 let h4 : handler rw [st_eq] a rw [st_eq3]
   = (| h4_raw , ((fun _ -> ()) , ()) |)
 
